tsrc/ZF_HOL.thy
@@ -34,24 +34,116 @@ thm GZF_HOL.un_iff
 find_consts "V"
 
 
-
-abbreviation tr3 where "tr3 G F A \<beta> \<equiv> transrec3 A F (\<lambda>\<alpha> f. G \<alpha> (VLambda \<alpha> f)) \<beta>"
 abbreviation ord where "ord x \<equiv> ZFC_in_HOL.Ord x"
 abbreviation lt where "lt x y \<equiv> x < y \<and> ord x \<and> ord y" 
+
 lemma succD : "ord (succ i) \<Longrightarrow> ord i"
   by (erule Ord_in_Ord, auto)
 
 
+lemma lt_ord : "lt i j \<Longrightarrow> ord i \<and> ord j" by auto
+lemma lt_mem : "lt i j \<Longrightarrow> mem i j" using lt_ord Ord_mem_iff_lt by auto
+lemma mem_lt : assumes "ord j" shows "mem i j \<Longrightarrow> lt i j" using OrdmemD assms Ord_in_Ord by auto
+
 (*Can't be proved automatically - might have to copy some of the development from Isabelle/ZF?*)
-lemma succ_iff : "i < succ j \<longleftrightarrow> i = j | (i < j & ord j)" sorry
+lemma succ_mem_iff : "i \<in> elts (succ j) \<longleftrightarrow> i \<in> elts j | i = j" 
+  unfolding elts_succ by auto
+
+lemma succ_iff : "lt i (succ j) \<longleftrightarrow> lt i j | i = j \<and> ord j"
+proof
+  assume "lt i (succ j)" hence mem:"mem i (succ j)" by (rule lt_mem)
+  have "ord i" "ord (succ j)" using lt_ord[OF \<open>lt i (succ j)\<close>] by auto
+  hence "ord j" using succD by auto
+  
+  from mem have "mem i j | i = j" using succ_mem_iff by auto
+  thus "lt i j | i = j \<and> ord j" using Ord_mem_iff_lt \<open>ord i\<close> \<open>ord j\<close> by auto
+next
+  assume "lt i j | i = j \<and> ord j"
+  thus "lt i (succ j)"
+  proof
+    assume "lt i j" hence "ord i" "ord j" by auto
+    from \<open>lt i j\<close> have "mem i j" using Ord_mem_iff_lt by auto
+    hence "mem i (succ j)" using succ_mem_iff by auto
+    hence "i < succ j" using Ord_mem_iff_lt[OF \<open>ord i\<close> Ord_succ[OF \<open>ord j\<close>]] by auto
+    thus "lt i (succ j)" using \<open>ord i\<close> \<open>ord j\<close>  by auto
+  next
+    assume h:"i = j \<and> ord j" 
+    hence "ord i" "ord (succ j)" using Ord_succ by auto
+
+    from h have "mem i (succ j)" using succ_mem_iff by auto
+    thus "lt i (succ j)" using Ord_mem_iff_lt[OF \<open>ord i\<close> \<open>ord (succ j)\<close>] \<open>ord i\<close> \<open>ord (succ j)\<close> by auto
+  qed
+qed
+
+lemma limit_iff : "\<forall>\<mu>. Limit \<mu> \<longleftrightarrow> (ord \<mu> \<and> lt 0 \<mu> \<and> (\<forall>\<beta>. lt \<beta> \<mu> \<longrightarrow> lt (succ \<beta>) \<mu>))" 
+  proof (rule, rule)
+    fix \<mu> assume "Limit \<mu>" hence def:"ord \<mu> \<and> mem 0 \<mu> \<and> (\<forall>y. mem y \<mu> \<longrightarrow> mem (ZFC_in_HOL.succ y) \<mu>)"
+      unfolding Limit_def by simp
+    hence 1: "ord \<mu>" and 2: "lt 0 \<mu>" using Ord_mem_iff_lt by auto
+    have 3: "(\<forall>\<beta>. lt \<beta> \<mu> \<longrightarrow> lt (succ \<beta>) \<mu>)" 
+    proof (rule, rule)
+      fix \<beta> assume "lt \<beta> \<mu>" hence "ord \<beta>" "mem \<beta> \<mu>" using Ord_mem_iff_lt by auto
+      hence "mem (succ \<beta>) \<mu>" using def by auto
+      thus "lt (succ \<beta>) \<mu>" using Ord_mem_iff_lt Ord_succ[OF \<open>ord \<beta>\<close>] \<open>ord \<mu>\<close> by auto
+    qed
+    from 1 2 3 show "ord \<mu> \<and> lt 0 \<mu> \<and> (\<forall>\<beta>. lt \<beta> \<mu> \<longrightarrow> lt (succ \<beta>) \<mu>)" by auto
+  next
+    fix \<mu> assume h:"ord \<mu> \<and> lt 0 \<mu> \<and> (\<forall>\<beta>. lt \<beta> \<mu> \<longrightarrow> lt (ZFC_in_HOL.succ \<beta>) \<mu>)"
+    thus "Limit \<mu>" unfolding Limit_def using lt_mem proof (auto)
+      fix y assume "mem y \<mu>" moreover hence "ord y" "ord \<mu>"using Ord_in_Ord h by auto
+      ultimately have "lt y \<mu>" using Ord_mem_iff_lt by auto
+      hence "lt (succ y) \<mu>" using h by auto
+      thus "mem (succ y) \<mu>" using lt_mem by auto
+    qed
+  qed
+
+lemma lt_trans : "lt i j \<Longrightarrow> lt j k \<Longrightarrow> lt i k" by auto
+lemma lt_notsym : "lt i j \<Longrightarrow> \<not> lt j i" by auto
+lemma lt_linear : "ord i \<and> ord j \<Longrightarrow> lt i j | i = j | lt j i" using Ord_linear_lt by auto
+lemma lt_induct : "ord a \<Longrightarrow> (\<And>x. ord x \<Longrightarrow> (\<And>y. lt y x \<Longrightarrow> P y) \<Longrightarrow> P x) \<Longrightarrow> P a"
+proof -
+  assume "ord a" "(\<And>x. ord x \<Longrightarrow> (\<And>y. lt y x \<Longrightarrow> P y) \<Longrightarrow> P x)"
+  hence "(\<And>x. ord x \<Longrightarrow> (\<And>y. mem y x \<Longrightarrow> P y) \<Longrightarrow> P x)" using lt_mem by auto
+  thus ?thesis by (rule Ord_induct[OF \<open>ord a\<close>])
+qed
+thm lt_mem
+lemma predset_def : "ord j \<Longrightarrow> mem i j \<longleftrightarrow> lt i j"
+  by (rule, rule mem_lt, use lt_mem in auto)
+
+
+(*Try using GZF_HOL.Lambda rather than VLambda*)
+abbreviation tr3 where "tr3 G F A \<beta> \<equiv> transrec3 A (\<lambda>i. F (succ i)) (\<lambda>\<alpha> f. G \<alpha> (VLambda \<alpha> f)) \<beta>"
+lemma rec0 : "tr3 G F A 0 = A" 
+ by (rule transrec3_0)
+
+lemma recsucc: "tr3 G F A (succ \<beta>) = F (succ \<beta>) (tr3 G F A \<beta>)"
+  by (rule transrec3_succ)
+thm GZF_HOL.upair_iff
+thm GZF_HOL.sng_iff
+
+lemma "vpair a b = GZF_HOL.kpair a b" proof
+  fix x show "mem x \<langle>a, b\<rangle> = mem x (GZF_HOL.kpair a b) " 
+  unfolding GZF_HOL.kpair_def using GZF_HOL.upair_iff vpair_def by auto
+qed
+
+lemma "VLambda x F = GZF_HOL.Lambda x F"
+lemma reclim : "Limit \<mu> \<Longrightarrow> tr3 G F A \<mu> = G \<mu> (GZF_HOL.Lambda \<mu> (\<lambda>b. tr3 G F A b))"
+  sorry
 
 interpretation Ord_HOL : Ord mem 0 "(\<lambda>x. True)" union subset VPow succ \<omega> repl
                              ord lt 0 succ Limit "(\<lambda>x. x)" tr3 \<omega>
 proof (unfold_locales)
   show "ord 0" by auto
   show "ord \<omega>" by auto
-  fix i j show "lt i j \<longrightarrow> ord i \<and> ord j" by auto
-  fix i j show "ord (succ i) \<longleftrightarrow> ord i" using Ord_in_Ord by auto
-  fix i show "\<not> lt i 0" by auto
-  show "\<forall>\<beta>. ord \<beta> \<longrightarrow> (\<forall>\<alpha>. lt \<alpha> (succ \<beta>) \<longleftrightarrow> (\<alpha> = \<beta> \<or> lt \<alpha> \<beta>))" using Ord_in_Ord by auto
+  show "\<forall>i j. lt i j \<longrightarrow> ord i \<and> ord j" using lt_ord by auto
+  show "\<forall>i. ord (succ i) \<longleftrightarrow> ord i" using Ord_in_Ord by auto
+  show "\<forall>i. \<not> lt i 0" by auto
+  show "(\<forall>\<alpha> \<beta>. lt \<alpha> (succ \<beta>) \<longleftrightarrow> (lt \<alpha> \<beta> | \<alpha> = \<beta>  \<and> ord \<beta>))" using succ_iff by simp
+  show "\<forall>\<mu>. Limit \<mu> \<longleftrightarrow> (ord \<mu> \<and> lt 0 \<mu> \<and> (\<forall>\<beta>. lt \<beta> \<mu> \<longrightarrow> lt (succ \<beta>) \<mu>))" by (rule limit_iff)
+  
 
+  
+  
+
+
+  
